Miniature_Five/LinearCode.thy
@@ -23,6 +23,10 @@ lemma elem_vs: "induced_vs F"
 
 definition W: "W = induced_vs.VS F n"
 lemma w_vs: "vectorspace F W" using induced_vs.vectorspace_VS elem_vs W by metis
+lemma w_carrier[simp]: "carrier W = words"
+  unfolding W induced_vs.VS[OF elem_vs, of n] words
+  using F_carrier
+  by simp
 
 lemma code_subspace: "subspace F C W" unfolding subspace_def using
     w_vs
@@ -36,6 +40,9 @@ lemma code_subspace: "subspace F C W" unfolding subspace_def using
   by auto
 
 abbreviation "CS" where "CS \<equiv> vectorspace.vs W C"
+corollary code_space: "vectorspace F CS"
+  using code_subspace w_vs vectorspace.subspace_is_vs
+  by metis
 
 lemma add_codeword_group: "group (add_monoid CS)"
   using module.submodule_is_module[of F W C] w_vs code_subspace vectorspace_def[of F W]
@@ -93,16 +100,6 @@ proof -
     using group_def[of "add_monoid CS"] add_codeword_group by simp
 qed
 
-lemma subtraction_closed:
-  assumes
-    "u \<in> C"
-    "v \<in> C"
-  shows
-    "u \<ominus>\<^bsub>CS\<^esub> v \<in> C"
-  unfolding a_minus_def
-  using assms inv_closed[OF assms(2)] abelian_monoid.a_closed[OF abelian_monoid_code]
-  by simp 
-
 lemma hamming_distance_subtract:
   assumes
     "u \<in> words"
@@ -110,12 +107,24 @@ lemma hamming_distance_subtract:
   shows
     "hamming_distance u v = hamming_distance \<zero>\<^bsub>W\<^esub> (u \<ominus>\<^bsub>W\<^esub> v)"
 proof -
-  have per_elem_equiv: "\<And>i. i \<in> {0..<n} \<Longrightarrow> (u$i \<noteq> v$i) = (\<zero>\<^bsub>W\<^esub>$i \<noteq> (u \<ominus>\<^bsub>W\<^esub> v)$i)" sorry
+  have per_elem_equiv: "\<And>i. i \<in> {0..<n} \<Longrightarrow> (u$i \<noteq> v$i) = (\<zero>\<^bsub>W\<^esub>$i \<noteq> (u \<ominus>\<^bsub>W\<^esub> v)$i)"
+    using assms
+    unfolding words
+    using induced_vs.elem_neq_dif_elem_nonzero[OF elem_vs] F_carrier
+    unfolding W
+    by presburger
 
-  have sub_word: "word (u \<ominus>\<^bsub>W\<^esub> v)" using subtraction_closed words_subs sorry
+  have sub_word: "word (u \<ominus>\<^bsub>W\<^esub> v)"
+    using vectorspace.subtraction_closed[OF w_vs] assms
+    by simp
 
-  have "\<zero>\<^bsub>W\<^esub> \<in> carrier W" sorry
-  have zero_word: "word \<zero>\<^bsub>W\<^esub>" sorry
+  have "\<zero>\<^bsub>W\<^esub> \<in> C"
+    using C_axioms(3)
+    unfolding W induced_vs.VS[OF elem_vs, of n]
+    by simp
+  then have zero_word: "word \<zero>\<^bsub>W\<^esub>"
+    using words_subs word
+    by blast
 
   have "hamming_distance u v = card {i \<in> {0..<n}. u$i \<noteq> v$i}"
     using assms word hamming_distance_def by presburger
@@ -142,10 +151,8 @@ proof -
 
       have "?u \<in> C" using p_props by force
       then have "?u \<in> words" using words_subs by force
-      from \<open>?u \<in> C\<close> have "?u \<in> carrier (add_monoid CS)" by simp
       have "?v \<in> C" using p_props by force
       then have "?v \<in> words" using words_subs by force
-      from \<open>?v \<in> C\<close> have "?v \<in> carrier (add_monoid CS)" by simp
 
       have carr: "carrier (add_monoid CS) = C" by simp
       from add_codeword_group have "monoid (add_monoid CS)" using group_def[of "add_monoid CS"] by fast
@@ -153,127 +160,19 @@ proof -
       have zero_equiv: "\<zero>\<^bsub>CS\<^esub> = \<zero>\<^bsub>W\<^esub>" unfolding W induced_vs.VS[OF elem_vs, of n] by simp
       have add_equiv: "add CS = add W" unfolding W by simp
       have scale_equiv: "module.smult CS = module.smult W" unfolding W by simp
-      have "\<And>u. u \<in> C \<Longrightarrow> \<ominus>\<^bsub>CS\<^esub> u = \<ominus>\<^bsub>W\<^esub> u" proof -
-        fix u
-        assume "u \<in> C"
-
-        have u_elems: "\<And>i. i \<in> {0..<n} \<Longrightarrow> u$i \<in> carrier F"
-          using \<open>u \<in> C\<close> words_subs words vec_set_def F_carrier by force
-
-        thm ring.ring_simprules
-
-        have "ring F" using field_F field_def domain_def cring_def by metis
-        then have "monoid F" using ring_def by metis
-
-        define v where v_def: "v = vec n (\<lambda>i. \<ominus>\<^bsub>F\<^esub> u$i)"
-        then have "v = vec n (\<lambda>i. \<ominus>\<^bsub>F\<^esub> (\<one>\<^bsub>F\<^esub> \<otimes>\<^bsub>F\<^esub> (u$i)))"
-          using monoid.l_one[OF \<open>monoid F\<close>] u_elems by auto
-        then have "v = vec n (\<lambda>i. (\<ominus>\<^bsub>F\<^esub> \<one>\<^bsub>F\<^esub>) \<otimes>\<^bsub>F\<^esub> (u$i))"
-          using ring.l_minus[OF \<open>ring F\<close> monoid.one_closed[OF \<open>monoid F\<close>]] u_elems
-          by auto
-        then have "v = (\<ominus>\<^bsub>F\<^esub> \<one>\<^bsub>F\<^esub>) \<odot>\<^bsub>W\<^esub> (vec n (\<lambda>i. u$i))"
-          unfolding W induced_vs.VS[OF elem_vs, of n]
-          using induced_vs.scaling_def[OF elem_vs, of n]
-          by auto
-        moreover have "dim_vec u = n" using \<open>u \<in> C\<close> words words_subs by blast
-        ultimately have "v = (\<ominus>\<^bsub>F\<^esub> \<one>\<^bsub>F\<^esub>) \<odot>\<^bsub>W\<^esub> u" using dim_vec eq_vecI index_vec
-          by metis
-        moreover have "(\<ominus>\<^bsub>F\<^esub> \<one>\<^bsub>F\<^esub>) \<in> carrier F"
-          using monoid.Units_closed[OF \<open>monoid F\<close>] ring.Units_minus_one_closed[OF \<open>ring F\<close>]
-          by presburger
-        ultimately have "v \<in> C" using C_axioms(2)[OF _ \<open>u \<in> C\<close>] F_carrier
-          unfolding W induced_vs.VS[OF elem_vs, of n]
-          by simp
-
-        have "ring F" using field_F field_def domain_def cring_def by metis
-
-        have "u \<oplus>\<^bsub>CS\<^esub> v = vec n (\<lambda>i. u$i \<oplus>\<^bsub>F\<^esub> v$i)"
-          unfolding W induced_vs.VS[OF elem_vs, of n]
-          using induced_vs.addition_def[OF elem_vs] by simp
-        also have "\<dots> = vec n (\<lambda>i. u$i \<oplus>\<^bsub>F\<^esub> (\<ominus>\<^bsub>F\<^esub> u$i))" using v_def by auto
-        also have "\<dots> = vec n (\<lambda>i. \<zero>\<^bsub>F\<^esub>)"
-          using ring.ring_simprules(16)[OF \<open>ring F\<close>] u_elems by auto
-        also have "\<dots> = \<zero>\<^bsub>CS\<^esub>"
-          unfolding W induced_vs.VS[OF elem_vs, of n]
-          using induced_vs.zero_vec_def[OF elem_vs]
-          by simp
-        finally have cs_sum: "u \<oplus>\<^bsub>CS\<^esub> v = \<zero>\<^bsub>CS\<^esub>" .
-        then have w_sum: "u \<oplus>\<^bsub>W\<^esub> v = \<zero>\<^bsub>W\<^esub>" using zero_equiv add_equiv by argo
-
-        have "v = \<ominus>\<^bsub>CS\<^esub> u" proof -
-          have "u \<in> Units (add_monoid CS)"
-            using all_invertible_CS[OF \<open>u \<in> C\<close>] .
-          moreover define w where w_inv: "w = \<ominus>\<^bsub>CS\<^esub> u"
-          then have "w \<oplus>\<^bsub>CS\<^esub> u = \<zero>\<^bsub>CS\<^esub>"
-            using monoid.Units_l_inv[OF \<open>monoid (add_monoid CS)\<close> \<open>u \<in> Units (add_monoid CS)\<close>]
-            unfolding a_inv_def m_inv_def
-            by auto
-          moreover from \<open>w = \<ominus>\<^bsub>CS\<^esub> u\<close> have "w \<in> C"
-            using monoid.Units_inv_closed[OF \<open>monoid (add_monoid CS)\<close> \<open>u \<in> Units (add_monoid CS)\<close>] a_inv_def[of CS]
-            by simp
-          ultimately have "v = w"
-            using monoid.inv_unique[OF \<open>monoid (add_monoid CS)\<close>, of w u v] cs_sum
-            using \<open>u \<in> C\<close> \<open>v \<in> C\<close> by auto
-          then show ?thesis using w_inv by presburger
-        qed
-        moreover have "v = \<ominus>\<^bsub>W\<^esub> u" proof -
-          from \<open>u \<in> C\<close> have "u \<in> words" using words_subs by blast
-          from \<open>v \<in> C\<close> have "v \<in> words" using words_subs by blast
-
-          have "carrier W = words"
-            unfolding W induced_vs.VS[OF elem_vs, of n]
-            using words F_carrier
-            by simp
-
-          have "monoid (add_monoid W)"
-            using w_vs
-            using vectorspace_def
-            using module_def abelian_group_def abelian_group_axioms_def
-            using comm_group_def[of "add_monoid W"] group_def
-            by blast
-
-          have "u \<in> Units (add_monoid W)"
-            using all_invertible_W[OF \<open>u \<in> words\<close>] .
-          moreover define w where w_inv: "w = \<ominus>\<^bsub>W\<^esub> u"
-          then have "w \<oplus>\<^bsub>W\<^esub> u = \<zero>\<^bsub>W\<^esub>"
-            using monoid.Units_l_inv[OF \<open>monoid (add_monoid W)\<close> \<open>u \<in> Units (add_monoid W)\<close>]
-            unfolding a_inv_def m_inv_def
-            by auto
-          moreover from \<open>w = \<ominus>\<^bsub>W\<^esub> u\<close> have "w \<in> words"
-            using monoid.Units_inv_closed[OF \<open>monoid (add_monoid W)\<close> \<open>u \<in> Units (add_monoid W)\<close>]
-            using a_inv_def[of W] \<open>carrier W = words\<close>
-            by auto
-          ultimately have "v = w"
-            using monoid.inv_unique[OF \<open>monoid (add_monoid W)\<close>, of w u v] cs_sum
-            using \<open>u \<in> words\<close> \<open>v \<in> words\<close> \<open>carrier W = words\<close> by auto
-          then show ?thesis using w_inv by presburger
-        qed
-        ultimately show "\<ominus>\<^bsub>CS\<^esub> u = \<ominus>\<^bsub>W\<^esub> u" by presburger
-      qed
+      have "\<And>u. u \<in> C \<Longrightarrow> \<ominus>\<^bsub>CS\<^esub> u = \<ominus>\<^bsub>W\<^esub> u"
+        using vectorspace.subspace_inverse_equal[OF w_vs code_subspace]
+        by presburger
       then have minus_equiv: "\<And>u v. u \<in> C \<Longrightarrow> v \<in> C \<Longrightarrow> u \<ominus>\<^bsub>CS\<^esub> v = u \<ominus>\<^bsub>W\<^esub> v"
         unfolding a_minus_def using \<open>add CS = add W\<close> by presburger
 
-      have "?u \<ominus>\<^bsub>CS\<^esub> ?v \<in> C" using subtraction_closed[OF \<open>?u \<in> C\<close> \<open>?v \<in> C\<close>] .
-      moreover have "(?u \<ominus>\<^bsub>CS\<^esub> ?v) \<noteq> \<zero>\<^bsub>CS\<^esub>" proof (rule ccontr)
-        assume "\<not> ?u \<ominus>\<^bsub>CS\<^esub> ?v \<noteq> \<zero>\<^bsub>CS\<^esub>"
-        then have eq_z: "?u \<oplus>\<^bsub>CS\<^esub> (\<ominus>\<^bsub>CS\<^esub> ?v) = \<zero>\<^bsub>CS\<^esub>" unfolding a_minus_def by simp
-        then have "inv\<^bsub>add_monoid CS\<^esub> (\<ominus>\<^bsub>CS\<^esub> ?v) = ?u"
-          using group.inv_equality[OF
-              \<open>group (add_monoid CS)\<close>
-              _
-              _
-              \<open>?u \<in> carrier (add_monoid CS)\<close>
-              ]
-          using inv_closed[OF \<open>?v \<in> C\<close>]
-          unfolding induced_vs.VS[OF elem_vs, of n] W
-          by auto
-        then have "inv\<^bsub>add_monoid CS\<^esub> (inv\<^bsub>add_monoid CS\<^esub> ?v) = ?u" using a_inv_def by metis
-        moreover have "?v \<in> Units (add_monoid CS)" using all_invertible_CS[OF \<open>?v \<in> C\<close>] .
-        ultimately have "?v = ?u"
-          using monoid.Units_inv_inv[OF \<open>monoid (add_monoid CS)\<close>]
-          by algebra
-        then show "False" using p_props by presburger
-      qed
+      have "?u \<ominus>\<^bsub>CS\<^esub> ?v \<in> C"
+        using vectorspace.subtraction_closed[OF code_space]
+        using \<open>?u \<in> C\<close> \<open>?v \<in> C\<close>
+        by simp
+      moreover have "(?u \<ominus>\<^bsub>CS\<^esub> ?v) \<noteq> \<zero>\<^bsub>CS\<^esub>" using vectorspace.eq_equiv_diff_zero[OF code_space, of ?u ?v]
+        using code_space \<open>?u \<in> C\<close> \<open>?v \<in> C\<close> p_props
+        by auto
 
       moreover from p_props have "x = hamming_distance \<zero>\<^bsub>CS\<^esub> (?u \<ominus>\<^bsub>CS\<^esub> ?v)"
         using words_subs hamming_distance_subtract[OF \<open>?u \<in> words\<close> \<open>?v \<in> words\<close>]
@@ -288,8 +187,8 @@ proof -
       assume "x \<in> {hamming_distance \<zero>\<^bsub>W\<^esub> w |w. w \<in> C \<and> w \<noteq> \<zero>\<^bsub>W\<^esub>}"
       then obtain w where w_props: "w \<in> C" "w \<noteq> \<zero>\<^bsub>W\<^esub>" "hamming_distance w \<zero>\<^bsub>W\<^esub> = x" by auto
       then have "(\<zero>\<^bsub>W\<^esub>, w) \<in> C \<times> C"
-        unfolding W induced_vs.VS
-        using elem_vs C_axioms induced_vs.VS
+        unfolding W
+        using elem_vs C_axioms
         by (simp add: induced_vs.VS)
       then show "x \<in> {hamming_distance (fst p) (snd p) |p. p \<in> C \<times> C \<and> fst p \<noteq> snd p}"
         using w_props
